Impl/StateSectorModel.i.dfy
@@ -16,28 +16,4 @@ module StateSectorModel {
     | SectorNode(node: Node)
     | SectorIndirectionTable(indirectionTable: IndirectionTableModel.IndirectionTable)
     | SectorSuperblock(superblock: SectorType.Superblock)
-
-  predicate WFSector(sector: Sector)
-  {
-    match sector {
-      case SectorNode(node) => BT.WFNode(node)
-      case SectorIndirectionTable(indirectionTable) => (
-        && IndirectionTableModel.Inv(indirectionTable)
-        && BC.WFCompleteIndirectionTable(IndirectionTableModel.I(indirectionTable))
-      )
-      case SectorSuperblock(superblock) =>
-        JC.WFSuperblock(superblock)
-    }
-  }
-
-  function ISector(sector: Sector) : SectorType.Sector
-  requires WFSector(sector)
-  {
-    match sector {
-      case SectorNode(node) => SectorType.SectorNode(BT.G.Node(node.pivotTable, node.children, node.buckets))
-      case SectorIndirectionTable(indirectionTable) =>
-        SectorType.SectorIndirectionTable(IndirectionTableModel.I(indirectionTable))
-      case SectorSuperblock(superblock) => SectorType.SectorSuperblock(superblock)
-    }
-  }
 }
